code/Yazi.Adler32.fst
@@ -1,0 +1,453 @@
+module Yazi.Adler32
+module B = LowStar.Buffer
+module Cast = FStar.Int.Cast
+module HS = FStar.HyperStack
+module Math = FStar.Math.Lemmas
+module ST = FStar.HyperStack.ST
+module U16 = FStar.UInt16
+module U32 = FStar.UInt32
+module U64 = FStar.UInt64
+module U8 = FStar.UInt8
+module UInt = FStar.UInt
+
+open FStar.Mul
+open FStar.Seq
+open Lib.UInt
+open LowStar.BufferOps
+open Spec.Adler32
+
+[@ CMacro ]
+let base64 = 65521UL
+let base_64_correct (_: unit): Lemma (ensures U64.v base64 == base) = ()
+
+[@ CMacro ]
+let nmax32 = 268961027ul
+let nmax32_correct (_: unit): Lemma (ensures U32.v nmax32 == nmax) = ()
+
+#set-options "--fuel 0 --ifuel 0"
+private noeq type do_init_state = {
+  dlen: nat;
+  data: input dlen;
+  blen: nat;
+  base: B.buffer U8.t;
+}
+
+private noeq type do_state = {
+  clen: Ghost.erased nat;
+  consumed: Ghost.erased (input clen);
+  slen: U32.t;
+  stream: B.buffer U8.t;
+  a: U64.t;
+  b: U64.t;
+}
+
+let sum_a_state (#n #m: nat) (data: input n) (consumed: input m) (a: U64.t) =
+ U64.v a == (sum_a data % base) + sum_seq consumed
+
+let sum_b_state (#n #m: nat) (data: input n) (consumed: input m) (b: U64.t) =
+ U64.v b == (sum_b data % base) + m * (sum_a data % base) + sum_b' consumed
+
+unfold let do_pre_cond (h: HS.mem) (d: do_init_state) (s: do_state) (steps: nat) =
+  B.live h d.base /\ B.length d.base == d.blen /\
+
+  s.clen + U32.v s.slen == d.blen /\ s.clen + steps <= nmax /\
+  Seq.equal (B.as_seq h d.base) (s.consumed @| (B.as_seq h s.stream)) /\
+  U32.v s.slen >= steps /\ B.live h s.stream /\ B.length s.stream == U32.v s.slen /\
+  sum_a_state d.data s.consumed s.a /\
+  sum_b_state d.data s.consumed s.b
+
+unfold let do_post_cond
+  (h0 h1: HS.mem)
+  (d: do_init_state)
+  (s: do_state)
+  (res: do_state)
+  (steps: nat) =
+  let sa = sum_a d.data % base in
+  do_pre_cond h0 d s steps /\
+  B.(modifies loc_none h0 h1) /\
+  Ghost.reveal res.clen == Seq.length res.consumed /\
+  res.clen + U32.v res.slen == d.blen /\
+  Seq.equal res.consumed (s.consumed @| (slice (B.as_seq h1 s.stream) 0 steps)) /\
+  Seq.equal (B.as_seq h1 d.base) (res.consumed @| (B.as_seq h1 res.stream)) /\
+  (U32.v res.slen == 0 ==> Seq.equal res.consumed (B.as_seq h1 d.base)) /\
+  
+  B.live h1 res.stream /\ B.length res.stream == U32.v res.slen /\
+  Seq.equal (slice (B.as_seq h1 s.stream) steps (U32.v s.slen)) (B.as_seq h1 res.stream) /\
+  sum_a_state d.data res.consumed res.a /\
+  sum_b_state d.data res.consumed res.b
+
+#set-options "--z3rlimit 1024 --fuel 0 --ifuel 0"
+let sum_a_state_mod
+  (#m1 #m2: nat)
+  (data: input m1)
+  (consumed: input m2)
+  (a: U64.t{sum_a_state data consumed a}): Lemma
+  (ensures U64.v a % base == (sum_a #(m1 + m2) (data @| consumed)) % base) =
+  calc (==) {
+    U64.v a % base;
+    =={}
+    ((sum_a data % base) + sum_seq consumed) % base;
+    =={Math.lemma_mod_plus_distr_l (sum_a data) (sum_seq consumed) base}
+    (sum_a data + sum_seq consumed) % base;
+    =={sum_a_append data consumed}
+    (sum_a #(m1 + m2) (data @| consumed)) % base;
+  }
+
+let sum_b_state_mod
+  (#m1 #m2: nat)
+  (data: input m1)
+  (consumed: input m2)
+  (b: U64.t{sum_b_state data consumed b}): Lemma
+  (ensures U64.v b % base == (sum_b #(m1 + m2) (data @| consumed)) % base) =
+  let sa = sum_a data % base in
+  calc (==) {
+    U64.v b % base;
+    =={}
+    ((sum_b data % base) + sum_b' consumed + m2 * sa) % base;
+    =={Math.paren_add_right (sum_b data % base) (sum_b' consumed) (m2 * sa)}
+    ((sum_b data % base) + (sum_b' consumed + m2 * sa)) % base;
+    =={Math.lemma_mod_add_distr (sum_b' consumed + m2 * sa) (sum_b data) base}
+    (sum_b data + sum_b' consumed + m2 * sa) % base;
+    =={Math.lemma_mod_add_distr (sum_b data + sum_b' consumed) (m2 * sa) base}
+    (sum_b data + sum_b' consumed + ((m2 * sa) % base)) % base;
+    =={Math.lemma_mod_mul_distr_r m2 (sum_a data) base}
+    (sum_b data + sum_b' consumed + ((m2 * sum_a data) % base)) % base;
+    =={Math.lemma_mod_add_distr (sum_b data + sum_b' consumed) (m2 * sum_a data) base}
+    (sum_b data + sum_b' consumed + m2 * sum_a data) % base;
+    =={sum_b_append data consumed}
+    (sum_b #(m1 + m2) (data @| consumed)) % base;
+  }
+
+inline_for_extraction
+let do1
+  (d: Ghost.erased do_init_state)
+  (s: do_state):
+  ST.Stack do_state
+  (requires fun h -> do_pre_cond h d s 1)
+  (ensures fun h0 res h1 -> do_post_cond h0 h1 d s res 1) =
+  let open U64 in
+  let sa = Ghost.hide (sum_a d.data % base) in
+  let byte = s.stream.(0ul) in
+  let byte' = Cast.uint8_to_uint64 byte in
+  let consumed' = Ghost.hide (snoc s.consumed byte) in
+
+  sum_a_seq_u64_upper_bound #_ #(s.clen + 1) d.data consumed';
+  let a' = s.a +^ byte' in
+  calc (==) {
+    v a';
+    =={}
+    v s.a + v byte';
+    =={
+      cast_zero_prefix (U8.v byte) 64;
+      zero_prefix_eq (v byte') (U8.v byte)
+    }
+    v s.a + U8.v byte;
+    =={}
+    sa + sum_seq s.consumed + U8.v byte;
+    =={sum_seq_append_byte s.consumed byte}
+    sa + sum_seq #(s.clen + 1) consumed';
+  };
+
+  calc (==) {
+    v s.b + v a';
+    =={}
+    (sum_b d.data % base) + s.clen * sa + sum_b' s.consumed +
+    sa + sum_seq #(s.clen + 1) (snoc s.consumed byte);
+    =={}
+    (sum_b d.data % base) + (s.clen + 1) * sa +
+    sum_b' s.consumed + sum_seq #(s.clen + 1) (snoc s.consumed byte);
+    =={sum_b'_sum_seq s.consumed byte}
+    (sum_b d.data % base) + (s.clen + 1) * sa + sum_b' #(s.clen + 1) (snoc s.consumed byte);
+    =={}
+    (sum_b d.data % base) + (s.clen + 1) * sa + sum_b' #(s.clen + 1) consumed';
+  };
+  sum_b'_u64_uppser_bound #_ #(s.clen + 1) d.data consumed';
+  let b' = s.b +^ a' in
+  {
+    clen = s.clen + 1;
+    consumed = consumed';
+    slen = U32.sub s.slen 1ul;
+    stream = B.sub s.stream 1ul (U32.sub s.slen 1ul);
+    a = a';
+    b = b';
+  }
+
+inline_for_extraction
+let rec iteration_1 (d: Ghost.erased do_init_state) (s: do_state): ST.Stack do_state
+  (requires fun h -> do_pre_cond h d s (U32.v s.slen) /\ d.blen <= nmax)
+  (ensures fun h0 res h1 -> do_post_cond h0 h1 d s res (d.blen - s.clen)) =
+  let open U32 in
+  if s.slen >^ 1ul then
+    let s' = do1 d s in
+    iteration_1 d s'
+  else if s.slen = 1ul then
+    do1 d s
+  else
+    s
+
+inline_for_extraction
+let rec iteration_1_remaining (d: Ghost.erased do_init_state) (s: do_state): ST.Stack do_state
+  (requires fun h -> do_pre_cond h d s (U32.v s.slen % 16) /\ d.blen <= nmax)
+  (ensures fun h0 res h1 -> do_post_cond h0 h1 d s res (U32.v s.slen % 16)) =
+  let open U32 in
+  if s.slen %^ 16ul >^ 0ul then
+    let s' = do1 d s in
+    iteration_1_remaining d s'
+  else
+    s
+
+inline_for_extraction
+let do2
+  (d: Ghost.erased do_init_state)
+  (s: do_state):
+  ST.Stack do_state
+  (requires fun h -> do_pre_cond h d s 2)
+  (ensures fun h0 res h1 -> do_post_cond h0 h1 d s res 2) =
+  let s' = do1 d s in
+  do1 d s'
+
+inline_for_extraction
+let do4
+  (d: Ghost.erased do_init_state)
+  (s: do_state):
+  ST.Stack do_state
+  (requires fun h -> do_pre_cond h d s 4)
+  (ensures fun h0 res h1 -> do_post_cond h0 h1 d s res 4) =
+  let s' = do2 d s in
+  do2 d s'
+
+inline_for_extraction
+let do8
+  (d: Ghost.erased do_init_state)
+  (s: do_state):
+  ST.Stack do_state
+  (requires fun h -> do_pre_cond h d s 8)
+  (ensures fun h0 res h1 -> do_post_cond h0 h1 d s res 8) =
+  let s' = do4 d s in
+  do4 d s'
+
+inline_for_extraction
+let do16
+  (d: Ghost.erased do_init_state)
+  (s: do_state):
+  ST.Stack do_state
+  (requires fun h -> do_pre_cond h d s 16)
+  (ensures fun h0 res h1 -> do_post_cond h0 h1 d s res 16) =
+  let s' = do8 d s in
+  do8 d s'
+
+inline_for_extraction
+let rec iteration_16 (d: Ghost.erased do_init_state) (s: do_state): ST.Stack do_state
+  (requires fun h ->
+    do_pre_cond h d s (U32.v s.slen) /\ U32.v s.slen % 16 == 0 /\ d.blen <= nmax)
+  (ensures fun h0 res h1 -> do_post_cond h0 h1 d s res (d.blen - s.clen)) =
+  let open U32 in
+  if s.slen >^ 16ul then
+    let s' = do16 d s in
+    iteration_16 d s'
+  else if s.slen = 16ul then
+    do16 d s
+  else
+    s
+
+inline_for_extraction
+let extract_sums
+  (#m: Ghost.erased nat)
+  (s: Ghost.erased (input m))
+  (adler: U32.t{adler32_matched s adler}):
+  Tot (adler32_pair s) =
+  let open U32 in
+  let a = adler &^ 0xfffful in
+  let sa: Ghost.erased (UInt.uint_t 16) = Ghost.hide ((sum_a s) % base) in
+  zero_prefix_eq (v a) sa;
+  
+  let b = adler >>^ 16ul in
+  let sb: Ghost.erased (UInt.uint_t 16) = Ghost.hide ((sum_b s) % base) in
+  zero_prefix_eq (v b) sb;
+  (Cast.uint32_to_uint64 a, Cast.uint32_to_uint64 b)
+
+#set-options "--z3rlimit 1024 --fuel 0 --ifuel 0 --z3seed 13"
+inline_for_extraction
+let combine_sums
+  (#m1 #m2: Ghost.erased nat)
+  (data: Ghost.erased (input m1))
+  (consumed: Ghost.erased (input m2))
+  (a: U64.t{sum_a_state data consumed a})
+  (b: U64.t{sum_b_state data consumed b}):
+  Tot (res: U32.t{adler32_matched #(m1 + m2) (data @| consumed) res}) =
+  let open U64 in
+  let sa = Ghost.hide (sum_a data % base) in
+  let a' = Cast.uint64_to_uint16 (a %^ base64) in
+  let a'' = Cast.uint16_to_uint32 a' in
+  sum_a_state_mod data consumed a;
+  cast_zero_prefix (U16.v a') 32;
+  assert(forall (i: nat{i < 32}).
+    (i < 16 ==> UInt.nth (U32.v a'') i == false) /\
+    (i >= 16 ==> UInt.nth (U32.v a'') i == UInt.nth (U16.v a') (i - 16)));
+
+  let b' = Cast.uint64_to_uint16 (b %^ base64) in
+  let b'' = Cast.uint16_to_uint32 b' in
+  sum_b_state_mod data consumed b;
+  cast_zero_prefix (U16.v b') 32;
+  assert(forall (i: nat{i < 32}).
+    (i < 16 ==> UInt.nth (U32.v b'') i == false) /\
+    (i >= 16 ==> UInt.nth (U32.v b'') i == UInt.nth (U16.v b') (i - 16)));
+  U32.logxor (U32.shift_left b'' 16ul) a''
+
+inline_for_extraction unfold let init_state'
+  (#m: Ghost.erased nat)
+  (data: Ghost.erased (input m))
+  (a': U64.t{sum_a_state #_ #0 data (Seq.empty #U8.t) a'})
+  (b': U64.t{sum_b_state #_ #0 data (Seq.empty #U8.t) b'})
+  (len: U32.t)
+  (buf: B.buffer U8.t{B.length buf == U32.v len}):
+  Tot ((Ghost.erased do_init_state) & do_state) =
+  (Ghost.hide ({
+    dlen = m;
+    data = data;
+    blen = U32.v len;
+    base = buf;
+  }), {
+    clen = 0;
+    consumed = Seq.empty #U8.t;
+    slen = len;
+    stream = buf;
+    a = a';
+    b = b';
+  })
+  
+inline_for_extraction unfold let init_state
+  (#m: Ghost.erased nat)
+  (data: Ghost.erased (input m))
+  (adler: U32.t{adler32_matched data adler})
+  (len: U32.t)
+  (buf: B.buffer U8.t{B.length buf == U32.v len}):
+  Tot ((Ghost.erased do_init_state) & do_state) =
+  let (a', b') = extract_sums data adler in
+  init_state' data a' b' len buf
+
+inline_for_extraction
+let rec do_iteration_nmax
+  (#m1 #m2: Ghost.erased nat)
+  (data: Ghost.erased (input m1))
+  (consumed: Ghost.erased (input m2))
+  (base_len: Ghost.erased nat{base_len >= nmax})
+  (base_buf: Ghost.erased (B.buffer U8.t){B.length base_buf == Ghost.reveal base_len})
+  (buf: B.buffer U8.t)
+  (r: U32.t)
+  (a b: U64.t):
+  ST.Stack (U64.t & U64.t & (B.buffer U8.t) & U32.t & (Ghost.erased (Seq.seq U8.t)))
+  (requires fun h ->
+    let r' = U32.v r in
+    let base_buf' = B.as_seq h base_buf in
+    let remaining = B.as_seq h buf in
+    B.live h base_buf /\ B.live h buf /\
+    B.length buf == r' /\ r' <= base_len /\ r' >= nmax /\
+    Seq.equal consumed (slice base_buf' 0 (base_len - r')) /\
+    Seq.equal (consumed @| remaining) base_buf' /\
+    (sum_a #(m1 + base_len - r') (data @| consumed)) % base == U64.v a /\
+    (sum_b #(m1 + base_len - r') (data @| consumed)) % base == U64.v b)
+  (ensures fun h0 res h1 ->
+    let (a', b', buf', r', consumed') = res in
+    let r'' = U32.v r' in
+    let base_buf' = B.as_seq h1 base_buf in
+    let remaining = B.as_seq h1 buf' in
+    B.(modifies loc_none h0 h1) /\
+    r'' < nmax /\ r'' == B.length buf' /\ B.live h1 buf' /\
+    Seq.equal consumed' (slice base_buf' 0 (base_len - r'')) /\
+    Seq.equal (consumed' @| remaining) base_buf' /\
+    (sum_a #(m1 + base_len - r'') (data @| consumed')) % base == U64.v a' /\
+    (sum_b #(m1 + base_len - r'') (data @| consumed')) % base == U64.v b') =
+  let open U32 in
+  let left = B.sub buf 0ul nmax32 in
+  let r' = r -^ nmax32 in
+  let right = B.sub buf nmax32 r' in
+  let (d, s) = init_state' #(m1 + m2) (data @| consumed) a b nmax32 left in
+  let s0 = iteration_1_remaining d s in
+  let s1 = iteration_16 d s0 in
+  let a' = U64.rem s1.a base64 in
+  calc (==) {
+    U64.v a';
+    =={}
+    U64.v s1.a % base;
+    =={sum_a_state_mod #(m1 + m2) #nmax (data @| consumed) s1.consumed s1.a}
+    (sum_a #(m1 + m2 + nmax) ((data @| consumed) @| s1.consumed)) % base;
+    =={append_assoc data consumed s1.consumed}
+    (sum_a #(m1 + m2 + nmax) (data @| (consumed @| s1.consumed))) % base;
+    =={}
+    (sum_a #(m1 + base_len - U32.v r') (data @| (consumed @| s1.consumed))) % base;
+  };
+  let b' = U64.rem s1.b base64 in
+  calc (==) {
+    U64.v b';
+    =={}
+    U64.v s1.b % base;
+    =={sum_b_state_mod #(m1 + m2) #nmax (data @| consumed) s1.consumed s1.b}
+    (sum_b #(m1 + m2 + nmax) ((data @| consumed) @| s1.consumed)) % base;
+    =={append_assoc data consumed s1.consumed}
+    (sum_b #(m1 + m2 + nmax) (data @| (consumed @| s1.consumed))) % base;
+    =={}
+    (sum_b #(m1 + base_len - U32.v r') (data @| (consumed @| s1.consumed))) % base;
+  };
+  if r' <^ nmax32 then
+    (a', b', right, r', (Ghost.hide (consumed @| s1.consumed)))
+  else
+    do_iteration_nmax #_ #(m2 + nmax)
+      data (consumed @| s1.consumed)
+      (base_len) (base_buf)
+      right r'
+      a' b'
+
+inline_for_extraction
+let iteration_nmax
+  (#m: Ghost.erased nat)
+  (data: Ghost.erased (input m))
+  (base: Ghost.erased (B.buffer U8.t))
+  (adler: U32.t{adler32_matched data adler})
+  (buf: B.buffer U8.t)
+  (len: U32.t):
+  ST.Stack (U32.t & (Ghost.erased (Seq.seq U8.t)))
+  (requires fun h ->
+    B.live h buf /\ B.length buf == U32.v len /\ U32.v len >= nmax)
+  (ensures fun h0 res h1 ->
+    let (adler', consumed) = res in
+    B.(modifies loc_none h0 h1) /\
+    Seq.equal consumed (data @| (B.as_seq h1 buf)) /\
+    adler32_matched #(m + U32.v len) (data @| (B.as_seq h1 buf)) adler') =
+  let open U32 in
+  append_empty_r data;
+  let (a, b) = extract_sums data adler in
+  let (a', b', buf', r', consumed) = do_iteration_nmax #_ #0
+    data (Seq.empty #U8.t)
+    (U32.v len) buf buf len
+    a b
+  in
+  let (d, s) = init_state'
+    #(m + v len - v r') (data @| consumed)
+    a' b'
+    r' buf'
+  in
+  let s' = iteration_1_remaining d s in
+  let s'' = iteration_16 d s' in
+  (combine_sums d.data s''.consumed s''.a s''.b, Ghost.hide (d.data @| s''.consumed))
+
+let adler32 #m data adler buf len =
+  let open U32 in
+  if len = 1ul then
+    let (d, s) = init_state data adler len buf in
+    let s' = do1 d s in
+    combine_sums data s'.consumed s'.a s'.b
+  else if len = 0ul then
+    adler
+  else if len <^ 16ul then
+    let (d, s) = init_state data adler len buf in
+    let s' = iteration_1 d s in
+    combine_sums data s'.consumed s'.a s'.b
+  else if len <=^ nmax32 then
+    let (d, s) = init_state data adler len buf in
+    let s' = iteration_1_remaining d s in
+    let s'' = iteration_16 d s' in
+    combine_sums data s''.consumed s''.a s''.b
+  else
+    let (adler', _) = iteration_nmax data buf adler buf len in
+    adler'
