code/Yazi.Adler32.fsti
@@ -1,0 +1,29 @@
+module Yazi.Adler32
+module B = LowStar.Buffer
+module Spec = Spec.Adler32
+module U32 = FStar.UInt32
+module U8 = FStar.UInt8
+module Seq = FStar.Seq
+module HS = FStar.HyperStack
+module ST = FStar.HyperStack.ST
+
+let empty_seq_aux (#a: Type) (h: HS.mem) (buf: B.buffer a) (s: Seq.seq a): Lemma
+  (requires B.length buf == 0)
+  (ensures Seq.append s (B.as_seq h buf) == s)
+  [SMTPat (Seq.append s (B.as_seq h buf))] =
+  assert(Seq.length (B.as_seq h buf) == 0);
+  Seq.lemma_empty (B.as_seq h buf);
+  Seq.append_empty_r s
+
+[@ (CPrologue "uint32_t adler32_z(uint32_t adler, const unsigned char *buf, size_t len);")]
+val adler32:
+    #m: Ghost.erased nat
+  -> data: Ghost.erased (Spec.input m)
+  -> adler: U32.t
+  -> buf: B.buffer U8.t
+  -> len: U32.t
+  -> ST.Stack U32.t
+  (requires fun h -> B.live h buf /\ B.length buf == U32.v len /\ Spec.adler32_matched data adler)
+  (ensures fun h0 res h1 ->
+    B.(modifies loc_none h0 h1) /\
+    Spec.adler32_matched #(m + U32.v len) (Seq.append data (B.as_seq h1 buf)) res)
