lib/Lib.Seq.fsti
@@ -1,0 +1,12 @@
+module Lib.Seq
+
+module Seq = FStar.Seq
+
+let unsnoc (#a: Type) (s: Seq.seq a{
+  Seq.length s > 0
+}): Tot (res: Seq.seq a{
+  (Seq.length res == Seq.length s - 1) /\
+  (forall (i: nat{i < Seq.length s - 1}).
+    Seq.index s i == Seq.index res i)
+}) =
+  Seq.slice s 0 (Seq.length s - 1)
