lib/Lib.UInt.fst
@@ -1,0 +1,115 @@
+module Lib.UInt
+
+module U32 = FStar.UInt32
+module UInt = FStar.UInt
+
+open FStar.Seq
+open FStar.Mul
+
+#set-options "--z3rlimit 120 --z3seed 1 --fuel 16 --ifuel 16"
+let rec cast_zero_prefix #n v m =
+  match m - n with
+  | 0 -> assert(Seq.equal (UInt.to_vec #m v) ((Seq.create (m - n) false) @| (UInt.to_vec v)))
+  | _ ->
+    if n >= 1 then
+      calc (==) {
+        UInt.to_vec #m v;
+        =={}
+        (UInt.to_vec #(m - 1) (v / 2)) @| (Seq.create 1 (v % 2 = 1));
+        =={
+          Math.Lemmas.pow2_le_compat (m - 1) (n - 1);
+          assert(v / 2 <= pow2 (n - 1));
+          cast_zero_prefix #(n - 1) (v / 2) (m - 1)
+        }
+        ((Seq.create (m - n) false) @| (UInt.to_vec #(n - 1) (v / 2))) @|
+        (Seq.create 1 (v % 2 = 1));
+        =={
+          Seq.append_assoc
+            (Seq.create (m - n) false)
+            (UInt.to_vec #(n - 1) (v / 2))
+            (Seq.create 1 (v % 2 = 1))
+        }
+        (Seq.create (m - n) false) @|
+        ((UInt.to_vec #(n - 1) (v / 2)) @| (Seq.create 1 (v % 2 = 1)));
+        =={}
+        (Seq.create (m - n) false) @| (UInt.to_vec v);
+      }
+    else begin
+      assert(Seq.equal (UInt.to_vec #m v) (Seq.create m false));
+      assert(UInt.to_vec #n v == Seq.empty #bool);
+      assert(Seq.equal (UInt.to_vec #m v) ((Seq.create m false) @| (Seq.empty #bool)))
+    end
+
+#set-options "--z3rlimit 200 --z3seed 1 --fuel 1 --ifuel 0"
+let div2_snoc (#n: nat{0 < n}) (a: UInt.uint_t n): Lemma
+  (ensures UInt.to_vec #(n - 1) (a / 2) == slice (UInt.to_vec a) 0 (n - 1)) =
+  calc (==) {
+    UInt.to_vec #(n - 1) (a / 2);
+    =={UInt.shift_right_value_lemma a 1}
+    UInt.to_vec #(n - 1) (UInt.shift_right a 1);
+    =={
+      assert(Seq.equal
+        (UInt.to_vec #(n - 1) (UInt.shift_right a 1))
+        (slice (UInt.to_vec a) 0 (n - 1)))
+    }
+    slice (UInt.to_vec a) 0 (n - 1);
+  }
+
+let rec zero_prefix_eq #n #m vn vm =
+  match m - n with
+  | 0 ->
+    assert(Seq.equal (UInt.to_vec vn) (UInt.to_vec vm));
+    UInt.to_vec_lemma_2 vm vn
+  | _ ->
+    let vm' = UInt.to_vec vm in
+    let vn' = UInt.to_vec vn in
+    match m with
+    | 1 ->
+      if last vm' then
+        UInt.to_vec_lemma_2 vn (UInt.one n)
+      else
+        UInt.to_vec_lemma_2 vn (UInt.zero n);
+      assert(vn == 1 \/ vn == 0);
+      calc (==) {
+        vm;
+        =={}
+        UInt.from_vec vm';
+        =={}
+        0 + (if last vm' then 1 else 0);
+        =={UInt.zero_from_vec_lemma #(n - 1)}
+        UInt.from_vec #(n - 1) (slice vn' 0 (n - 1)) + (if last vn' then 1 else 0);
+        =={}
+        UInt.from_vec vn';
+        =={UInt.inverse_num_lemma vn}
+        vn;
+      }
+    | _ ->
+      let vm'' = slice vm' 0 (m - 1) in
+      let vn'' = slice vn' 0 (n - 1) in
+      div2_snoc vm;
+      div2_snoc vn;
+      zero_prefix_eq #(n - 1) #(m - 1) (vn / 2) (vm / 2);
+      calc (==) {
+        vm;
+        =={}
+        UInt.from_vec vm';
+        =={}
+        2 * (UInt.from_vec #(m - 1) vm'') + (if last vm' then 1 else 0);
+        =={div2_snoc vm}
+        2 * (UInt.from_vec (UInt.to_vec #(m - 1) (vm / 2))) + (if last vn' then 1 else 0);
+        =={}
+        2 * (vn / 2) + (if last vn' then 1 else 0);
+        =={}
+        vn;
+      }
+
+#set-options "--z3rlimit 200 --ifuel 128 --fuel 128 --z3seed 1"
+let logand_256 r =
+  let open U32 in
+  let mask = v 0xFFul in
+  assert(forall (i: nat{i < 32}).
+    (i < 32 - 8 ==> UInt.nth mask i == false) /\
+    (i >= 32 - 8 ==> UInt.nth mask i == true));
+  assert(forall (i: nat{i < 32}).
+    (i < 32 - 8 ==> UInt.nth (UInt.logand (v r) (v 0xFFul)) i == false) /\
+    (i >= 32 - 8 ==> UInt.nth (UInt.logand (v r) (v 0xFFul)) i == UInt.nth (U32.v r) i))
