lib/Lib.UInt.fsti
@@ -1,0 +1,81 @@
+module Lib.UInt
+
+module U32 = FStar.UInt32
+module UInt = FStar.UInt
+module Seq = FStar.Seq
+
+#set-options "--z3rlimit 120 --z3seed 1 --fuel 16 --ifuel 16"
+val cast_zero_prefix:
+    #n: nat
+  -> v: UInt.uint_t n
+  -> m: nat{m >= n}
+  -> Lemma
+  (requires pow2 n <= pow2 m)
+  (ensures UInt.to_vec #m v == Seq.append (Seq.create (m - n) false) (UInt.to_vec v))
+
+val zero_prefix_eq:
+    #n: nat{0 < n}
+  -> #m: nat{0 < m /\ m <= n}
+  -> vn: UInt.uint_t n
+  -> vm: UInt.uint_t m
+  -> Lemma
+  (requires forall (i: nat{i < n}).
+    (i < n - m ==> UInt.nth vn i == false) /\
+    (n - m <= i ==> UInt.nth vn i == UInt.nth vm (i - n + m)))
+  (ensures vn == vm)
+
+val logand_256: (r: U32.t) -> Lemma
+  (ensures forall (i: nat{i < 32}).
+    (i < 32 - 8 ==> UInt.nth (U32.v (U32.logand r 0xFFul)) i == false) /\
+    (i >= 32 - 8 ==> UInt.nth (U32.v (U32.logand r 0xFFul)) i == UInt.nth (U32.v r) i))
+
+let rec uint_one_vec (#n: nat{n > 0}) (v: UInt.uint_t n): Lemma
+  (requires v == 1)
+  (ensures forall i. {:pattern UInt.nth v i}
+    (i == n - 1 ==> UInt.nth #n v i == true) /\
+    (i < n - 1 ==> UInt.nth #n v i == false)) =
+  match n with
+  | 1 -> ()
+  | _ -> uint_one_vec #(n - 1) v
+
+let mask_bit_status (#n: nat{n > 0}) (s: nat{s < n}) (v: UInt.uint_t n): Lemma
+  (requires v == UInt.shift_left 1 s)
+  (ensures forall j. {:pattern UInt.nth v j}
+    (j == n - 1 - s ==> UInt.nth v j == true) /\
+    (j <> n - 1 - s ==> UInt.nth v j == false)) =
+  uint_one_vec #n 1
+
+let mask_logor_status (#n: nat{n > 0}) (s: nat{s < n}) (mask v: UInt.uint_t n): Lemma
+  (requires mask == UInt.shift_left 1 s /\ UInt.nth v (n - 1 - s) == false)
+  (ensures
+    forall j. {:pattern UInt.nth (UInt.logor v mask) j}
+    (j <> n - 1 - s ==> UInt.nth (UInt.logor v mask) j == UInt.nth v j) /\
+    (j == n - 1 - s ==> UInt.nth (UInt.logor v mask) j == true)) =
+  mask_bit_status s mask
+
+let mask_logand_status (#n: nat{n > 0}) (s: nat{s < n}) (mask v: UInt.uint_t n): Lemma
+  (requires mask == UInt.shift_left 1 s)
+  (ensures
+    forall j. {:pattern UInt.nth (UInt.logand v mask) j}
+    (j <> n - 1 - s ==> UInt.nth (UInt.logand v mask) j == false) /\
+    (j == n - 1 - s ==> UInt.nth (UInt.logand v mask) j == (UInt.nth v (n - 1 - s) = true))) =
+  mask_bit_status s mask
+
+#set-options "--fuel 1 --ifuel 1"
+let logand_one_ne (#n: nat{n > 0}) (a: UInt.uint_t n): Lemma
+  (requires UInt.logand a (UInt.one n) <> 1)
+  (ensures UInt.logand a (UInt.one n) == 0) =
+  let one = UInt.one n in
+  let s = UInt.logand a one in
+  uint_one_vec one;
+  assert(forall i. i < n - 1 ==> UInt.nth s i == false);
+  if UInt.nth (UInt.logand a one) (n - 1) then
+    UInt.nth_lemma s one
+  else
+    UInt.nth_lemma s (UInt.zero n)
+
+#set-options "--z3rlimit 120 --fuel 128 --ifuel 128 --z3seed 13"
+let one_shift_left (s: U32.t{U32.v s < 32}): Lemma
+  (ensures forall (i: nat{i < 32}).
+    (i == 31 - U32.v s ==> UInt.nth (U32.v (U32.shift_left 1ul s)) i == true) /\
+    (i <> 31 - U32.v s ==> UInt.nth (U32.v (U32.shift_left 1ul s)) i == false)) = ()
