specs/Spec.Adler32.fst
@@ -1,0 +1,273 @@
+module Spec.Adler32
+
+module U8 = FStar.UInt8
+module Math = FStar.Math.Lemmas
+
+open FStar.Mul
+open FStar.Seq
+open Lib.Seq
+
+let rec sum_a_upper_bound_aux #n s =
+  match n with
+  | 0 -> ()
+  | _ -> sum_a_upper_bound_aux #(n - 1) (tail s)
+
+let rec sum_seq_append_byte #m s b =
+  match m with
+  | 0 -> ()
+  | _ ->
+    calc (==) {
+      sum_seq s + U8.v b;
+      =={}
+      U8.v (head s) + sum_seq #(m - 1) (tail s) + U8.v b;
+      =={sum_seq_append_byte #(m - 1) (tail s) b}
+      U8.v (head s) + sum_seq #m (snoc (tail s) b);
+      =={}
+      U8.v (head (create 1 (head s))) + sum_seq #m (snoc (tail s) b);
+      =={
+        lemma_head_append (create 1 (head s)) (snoc (tail s) b);
+        lemma_tail_append (create 1 (head s)) (snoc (tail s) b);
+        assert(equal
+          ((tail (create 1 (head s))) @| (snoc (tail s) b))
+          (snoc (tail s) b))
+      }
+      sum_seq #(m + 1) ((create 1 (head s)) @| (snoc (tail s) b));
+      =={
+         assert(equal
+           ((create 1 (head s)) @| (snoc (tail s) b))
+           (snoc s b))
+      }
+      sum_seq #(m + 1) (snoc s b);
+    }
+    
+#set-options "--z3rlimit 200 --fuel 1 --ifuel 1"
+let rec sum_a_append #m1 #m2 s1 s2 =
+  let open U8 in
+  match m1 with
+  | 0 ->
+    calc (==) {
+      sum_a #(m1 + m2) (s1 @| s2);
+      =={
+        Seq.lemma_empty s1;
+        Seq.append_empty_l s2
+      }
+      sum_a s2;
+      =={}
+      1 + sum_seq s2;
+      =={}
+      sum_a s1 + sum_seq s2;
+    }
+  | _ ->
+    calc (==) {
+      sum_a #(m1 + m2) (s1 @| s2);
+      =={}
+      1 + sum_seq #(m1 + m2) (s1 @| s2);
+      =={
+        lemma_head_append s1 s2;
+        Seq.lemma_tail_append s1 s2
+      }
+      1 + U8.v (head s1) + sum_seq #(m1 + m2 - 1) ((tail s1) @| s2);
+      =={}
+      U8.v (head s1) + sum_a #(m1 + m2 - 1) ((tail s1) @| s2);
+      =={sum_a_append #(m1 - 1) #m2 (tail s1) s2}
+      U8.v (head s1) + sum_a #(m1 - 1) (tail s1) + sum_seq s2;
+      =={}
+      sum_a s1 + sum_seq s2;
+    }
+
+#set-options "--z3rlimit 65536 --fuel 1 --ifuel 0 --z3seed 49999"
+let rec sum_b'_append (#m1 #m2: nat) (s1: input m1) (s2: input m2): Lemma (ensures
+  sum_b' #(m1 + m2) (Seq.append s1 s2) == sum_b' s1 + m2 * (sum_seq s1) + sum_b' s2) =
+  let open U8 in
+  match m1 with
+  | 0 -> 
+    calc (==) {
+      sum_b' s1 + m2 * (sum_seq s1) + sum_b' s2;
+      =={}
+      m2 * (sum_seq s1) + sum_b' s2;
+      =={}
+      sum_b' s2;
+      =={
+         Seq.lemma_empty s1;
+         Seq.append_empty_l s2
+      }
+      sum_b' #(m1 + m2) (s1 @| s2);
+    }
+  | _ ->
+    calc (==) {
+      sum_b' #(m1 + m2) (s1 @| s2);
+      =={}
+      (m1 + m2) * (v (head (s1 @| s2))) + sum_b' #(m1 + m2 - 1) (tail (s1 @| s2));
+      =={Seq.lemma_tail_append s1 s2}
+      (m1 + m2) * (v (head (s1 @| s2))) + sum_b' #(m1 + m2 - 1) ((tail s1) @| s2);
+      =={Seq.lemma_head_append s1 s2}
+      (m1 + m2) * (v (head s1)) + sum_b' #(m1 + m2 - 1) ((tail s1) @| s2);
+      =={sum_b'_append #(m1 - 1) #m2 (tail s1) s2}
+      (m1 + m2) * (v (head s1)) +
+      sum_b' #(m1 - 1) (tail s1) +
+      m2 * sum_seq #(m1 - 1) (tail s1) +
+      sum_b' s2;
+      =={}
+      m1 * (v (head s1)) +
+      sum_b' #(m1 - 1) (tail s1) +
+      m2 * (v (head s1)) +
+      m2 * sum_seq #(m1 - 1) (tail s1) +
+      sum_b' s2;
+      =={}
+      sum_b' s1 + m2 * sum_seq s1 + sum_b' s2;
+    }
+
+let rec sum_a_sum_seq (#m: nat) (s: input m): Lemma
+  (ensures sum_a s - 1 == sum_seq s) =
+  let open U8 in
+  match m with
+  | 0 -> ()
+  | _ ->
+    calc (==) {
+      sum_a s - 1;
+      =={}
+      v (head s) + sum_a #(m - 1) (tail s) - 1;
+      =={sum_a_sum_seq #(m - 1) (tail s)}
+      v (head s) + sum_seq #(m - 1) (tail s);
+      =={}
+      sum_seq s;
+    }
+
+let sum_b_append #m1 #m2 s1 s2 =
+  calc (==) {
+    sum_b #(m1 + m2) (s1 @| s2);
+    =={}
+    sum_b' #(m1 + m2) (s1 @| s2) + m1 + m2;
+    =={sum_b'_append s1 s2}
+    sum_b' s1 + m2 * (sum_seq s1) + sum_b' s2 + m1 + m2;
+    =={sum_a_sum_seq s1}
+    sum_b' s1 + m2 * (sum_a s1 - 1) + sum_b' s2 + m1 + m2;
+    =={}
+    sum_b' s1 + m2 * sum_a s1 + sum_b' s2 + m1;
+    =={}
+    sum_b s1 + m2 * sum_a s1 + sum_b' s2;
+  }
+
+let n_mod2_aux (n: nat{n > 0}): Lemma
+  (ensures (n * (n - 1)) % 2 == 0) =
+  if n % 2 = 0 then
+    calc (==) {
+      (n * (n - 1)) % 2;
+      =={Math.div_exact_r n 2}
+      (2 * (n / 2) * (n - 1)) % 2;
+      =={Math.paren_mul_right 2 (n / 2) (n - 1)}
+      (2 * ((n / 2) * (n - 1))) % 2;
+      =={Math.cancel_mul_mod ((n / 2) * (n - 1)) 2}
+      0;
+    }
+  else
+    calc (==) {
+      (n * (n - 1)) % 2;
+      =={Math.div_exact_r (n - 1) 2}
+      (n * (((n - 1) / 2) * 2)) % 2;
+      =={Math.paren_mul_right n ((n - 1) / 2) 2}
+      (n * ((n - 1) / 2) * 2) % 2;
+      =={Math.cancel_mul_mod (n * ((n - 1) / 2)) 2}
+      0;
+    }
+
+let rec sum_b_upper_bound_aux #n s =
+  match n with
+  | 0 -> ()
+  | _ ->
+    calc (<=) {
+      sum_b s;
+      =={assert(Seq.equal s ((create 1 (head s)) @| tail s))}
+      sum_b #n ((create 1 (head s)) @| tail s);
+      =={sum_b_append #1 #(n - 1) (create 1 (head s)) (tail s)}
+      sum_b #1 (create 1 (head s)) +
+      (n - 1) * sum_a #1 (create 1 (head s)) +
+      sum_b #(n - 1) (tail s) - n + 1;
+      =={assert_norm(sum_b #1 (create 1 (head s)) == (U8.v (head s)) + 1)}
+      (U8.v (head s)) + 1 +
+      (n - 1) * (U8.v (head s) + 1) +
+      sum_b #(n - 1) (tail s) - n + 1;
+      =={}
+      1 + n * (U8.v (head s)) + sum_b #(n - 1) (tail s);
+      <= {sum_b_upper_bound_aux #(n - 1) (tail s)}
+      1 + n * (U8.v (head s)) + (1 + (n - 1)) * (n - 1) * 255/ 2 + (n - 1);
+      <={}
+      n * 255 + n * (n - 1) * 255 / 2 + n;
+      =={Math.swap_mul (n - 1) 255}
+      n * 255 + n * 255 * (n - 1) / 2 + n;
+      =={}
+      (n * 255 + n * 255 * (n - 1) / 2 + n) * 2 / 2;
+      =={
+        calc (==) {
+          (n * 255 * (n - 1)) % 2;
+          =={Math.swap_mul 255 (n - 1)}
+          (n * (n - 1) * 255) % 2;
+          =={Math.lemma_mod_mul_distr_l (n * (n - 1)) 255 2}
+          (((n * (n - 1)) % 2) * 255) % 2;
+          =={n_mod2_aux n}
+          0;
+        };
+        Math.div_exact_r (n * 255 * (n - 1)) 2
+      }
+      (n * 255 * 2 + n * 255 * (n - 1) + n * 2) / 2;
+      =={}
+      (n * 255 * (n + 1) + n * 2) / 2;
+      =={}
+      n * 255 * (n + 1) / 2 + n;
+      =={Math.swap_mul 255 (n + 1)}
+      n * (n + 1) * 255 / 2 + n;
+      =={}
+      sum_b_upper_bound n;
+    }
+
+#set-options "--fuel 0 --ifuel 0"
+let rec sum_b'_sum_seq #m s byte =
+  match m with
+  | 0 -> ()
+  | _ ->
+    calc (==) {
+      sum_b' s + sum_seq #(m + 1) (snoc s byte);
+      =={}
+      m * (U8.v (head s)) + sum_b' #(m - 1) (tail s) +
+      sum_seq #(m + 1) (snoc s byte);
+      =={
+        lemma_head_append s (create 1 byte);
+        lemma_tail_append s (create 1 byte)
+      }
+      m * (U8.v (head s)) + sum_b' #(m - 1) (tail s) +
+      U8.v (head s) + sum_seq #m (snoc (tail s) byte);
+      =={}
+      (m + 1) * (U8.v (head s)) + sum_b' #(m - 1) (tail s) +
+      sum_seq #m (snoc (tail s) byte);
+      =={sum_b'_sum_seq #(m - 1) (tail s) byte}
+      (m + 1) * (U8.v (head s)) + sum_b' #m (snoc (tail s) byte);
+      =={
+        lemma_head_append (create 1 (head s)) (snoc (tail s) byte);
+        lemma_tail_append (create 1 (head s)) (snoc (tail s) byte);
+        append_empty_r (snoc (tail s) byte);
+        assert(equal
+          (tail ((create 1 (head s)) @| snoc (tail s) byte))
+          (snoc (tail s) byte))
+      }
+      sum_b' #(m + 1) ((create 1 (head s)) @| snoc (tail s) byte);
+      =={
+        assert(equal
+          ((create 1 (head s)) @| (snoc (tail s) byte))
+          (snoc s byte))
+      }
+      sum_b' #(m + 1) (snoc s byte);
+    }
+
+let sum_b'_u64_uppser_bound #n #m s c =
+  calc (<=) {
+     (sum_b s % base) + m * (sum_a s % base) + sum_b' c;
+     <={
+       Math.modulo_range_lemma (sum_b s) base;
+       Math.modulo_range_lemma (sum_a s) base
+     }
+     (base - 1) + m * (base - 1) + sum_b' c;
+     <={sum_b'_upper_bound_aux c}
+     1 * (base - 1) + m * (base - 1) + ((sum_b_upper_bound m) - m);
+     =={Math.distributivity_add_left 1 m (base - 1)}
+     (m + 1) * (base - 1) + m * (m + 1) * 255 / 2;
+  }
