Makefile
@@ -152,7 +152,7 @@ KRML=$(KREMLIN_HOME)/krml
 # easily turn this file into a .h, use -add-include '"Impl_Bignum_Intrinsics.h"'
 # and pass -static-header Impl.Bignum.Intrinsics as described in the
 # documentation.
-HAND_WRITTEN_C_FILES = code/c/Yazi_Allocator.h code/c/Yazi_Z_Stream_Fields.inc code/c/Yazi_CRC32_Table_Codegen.c
+HAND_WRITTEN_C_FILES = code/c/Yazi_Allocator.h code/c/Yazi_Z_Stream_Fields.inc code/c/Yazi_Adler32_Z.inc
 
 # This is now the preferred and recommended way to compile C code with KreMLin.
 #
@@ -180,7 +180,8 @@ dist/Makefile.basic: $(filter-out %prims.krml,$(ALL_KRML_FILES)) $(HAND_WRITTEN_
 	$(KRML) -tmpdir $(dir $@) -skip-compilation \
 	  $(filter %.krml,$^) \
 	  -warn-error @4@5@18 \
-	  -drop LowStar.ConstBuffer,C.Loops,Spec.*,Prims\
+	  -drop LowStar.ConstBuffer,C.Loops,Spec.*,Prims,Lib.*\
+	  -no-prefix Yazi.Adler32 \
 	  -no-prefix Yazi.CRC32_Table \
 	  -no-prefix Yazi.Util \
 	  -no-prefix Yazi.CFlags \
@@ -194,7 +195,12 @@ dist/Makefile.basic: $(filter-out %prims.krml,$(ALL_KRML_FILES)) $(HAND_WRITTEN_
 	  -add-early-include '"Yazi_Allocator.h"' \
 	  -add-include '"kremlin/internal/target.h"' \
 	  -o libz.a
-	  sed -i '/deflate_state \*state;.*/a #include "Yazi_Z_Stream_Fields.inc"' dist/Yazi_Types.h
+	sed -i \
+          '/deflate_state \*state;.*/a #include "Yazi_Z_Stream_Fields.inc"' \
+	  dist/Yazi_Types.h
+	sed -i \
+          '/adler32_z/c\#include "Yazi_Adler32_Z.inc"' \
+	  dist/Yazi_Adler32.c
 
 # Compiling the generated C code
 # ------------------------------
@@ -208,9 +214,13 @@ crc32_table_gen: dist/Makefile.basic
 	cc -I ./dist \
 	   -I $(KREMLIN_HOME)/include \
 	   -I $(KREMLIN_HOME)/kremlib/dist/minimal \
-	   dist/Yazi_CRC32_Table_Codegen.c dist/Yazi_CRC32_Table.c dist/Yazi_CRC32_Impl.c\
+	   code/c/Yazi_CRC32_Table_Codegen.c dist/Yazi_CRC32_Table.c dist/Yazi_CRC32_Impl.c\
 	   -o ./dist/crc32_table_gen
-	./dist/crc32_table_gen >> ./dist/Yazi_CRC32_Impl.c
+	./dist/crc32_table_gen > ./dist/Yazi_CRC32_Impl_Table.inc
+	sed -i \
+          '/crc32_combine64/c\#include "Yazi_CRC32_Impl_Table.inc"' \
+	  dist/Yazi_CRC32_Impl.c
+	rm ./dist/crc32_table_gen
 
 dist/libz.a: dist/Makefile.basic crc32_table_gen
 	$(MAKE) -C $(dir $@) -f $(notdir $<)
